except mem read and bitvec composition

SP1Chips/Load/LoadWord.lean
@@ -1,5 +1,6 @@
 import SP1Foundations
 import SP1Chips.Load.LoadWord.Constraints
+import SP1Operations.Operation.AddrAddOperation
 import LeanRV64IM.Specialization
 import LeanRV64IM.RiscvMem
 import LeanRV64IM.RiscvInstsEnd
@@ -67,7 +68,7 @@ def sp1_lw : SailM ExecutionResult :=
   do
     let op_a := sp1_op_a Main cstrs h_is_lw
     Sail.writeReg Register.nextPC (Word.toBitVec64 #v[Main[3] + 4, Main[4], Main[5], 0])
-    Sail.write_reg op_a (Word.toBitVec64 #v[Main[39], Main[40], Main[41] * 65536, Main[42] * 65536])
+    Sail.write_reg op_a (Word.toBitVec64 #v[Main[39], Main[40], Main[41] * 65536, Main[41] * 65536])
     pure RETIRE_SUCCESS
 
 attribute [simp] bind StateT.bind ExceptT.bind EStateM.bind ExceptT.bindCont get getThe MonadStateOf.get StateT.get EStateM.get pure StateT.pure ExceptT.pure EStateM.pure Functor.map StateT.map ExceptT.map EStateM.map modify modifyGet EStateM.modifyGet StateT.modifyGet MonadStateOf.modifyGet liftM monadLift MonadLift.monadLift ExceptT.lift StateT.lift ExceptT.mk StateT.run ExceptT.run EStateM.run Sail.SailME.run
@@ -92,22 +93,42 @@ theorem correct
     extract_lets op_a op_b op_c
     have h_not_lwu : Main[43] = 0 := is_lw_eq_not_lwu Main cstrs h_is_lw
 
-    simp [constraints, AddressOperation.constraints, AddrAddOperation.constraints, U16MSBOperation.constraints, CPUState.constraints, ITypeReader.constraints, SP1Constraint.toStateProp, List.Forall, h_is_lw, h_not_lwu, Opcode.ofNat, ByteOpcode.ofNat, Nat.beq, Nat.ble] at state_cstrs
-    obtain ⟨h_read_pc, h_read_op_a', h_read_op_b', h_read_mem⟩ := state_cstrs
+    simp [-Word.add_toBitVec64_mod4, constraints, AddressOperation.constraints, AddrAddOperation.constraints, U16MSBOperation.constraints, CPUState.constraints, ITypeReader.constraints, SP1Constraint.toStateProp, List.Forall, h_is_lw, h_not_lwu, Opcode.ofNat, ByteOpcode.ofNat, Nat.beq, Nat.ble] at state_cstrs
+    obtain ⟨h_read_pc, h_trusted_read, h_read_op_a, h_read_op_b, h_read_mem⟩ := state_cstrs
+
+    simp [constraints, AddressOperation.constraints, SP1Constraint.toProp, List.Forall, h_is_lw, h_not_lwu, Opcode.ofNat, ByteOpcode.ofNat, Nat.beq, Nat.ble, sub_eq_zero] at cstrs
+    obtain ⟨addr_add_cstrs, addr_cstr0, addr_cstr1, addr_cstr2, msb_cstrs, cpu_cstrs, reader_cstrs, chip_cstrs⟩ := cstrs
 
     have h_op_a_is_reg : Main[6] < 32 :=
       by
-        simp [constraints, AddressOperation.constraints, AddrAddOperation.constraints, CPUState.constraints, ITypeReader.constraints, SP1Constraint.toProp, List.Forall, h_is_lw, h_not_lwu, Opcode.ofNat, ByteOpcode.ofNat, Nat.beq, Nat.ble] at cstrs
+        simp [ITypeReader.constraints, SP1Constraint.toProp, List.Forall, h_is_lw, h_not_lwu, Opcode.ofNat, ByteOpcode.ofNat, Nat.beq, Nat.ble] at reader_cstrs
         simp_all only
-    have h_read_op_a := h_read_op_a' h_op_a_is_reg
-    clear h_read_op_a'
+    simp [h_op_a_is_reg] at h_read_op_a
     have h_op_b_is_reg : Main[14] < 32 :=
       by
-        simp [constraints, AddressOperation.constraints, AddrAddOperation.constraints, CPUState.constraints, ITypeReader.constraints, SP1Constraint.toProp, List.Forall, h_is_lw, h_not_lwu, Opcode.ofNat, ByteOpcode.ofNat, Nat.beq, Nat.ble] at cstrs
+        simp [ITypeReader.constraints, SP1Constraint.toProp, List.Forall, h_is_lw, h_not_lwu, Opcode.ofNat, ByteOpcode.ofNat, Nat.beq, Nat.ble] at reader_cstrs
         simp_all only
-    have h_read_op_b := h_read_op_b' h_op_b_is_reg
-    clear h_read_op_b'
+    simp [h_op_b_is_reg] at h_read_op_b
+    -- simp [-Word.add_toBitVec64_mod4, ←BitVec.ofNatLT_eq_ofNat (w := 5) (n := Main[14].val) h_op_b_is_reg, h_read_op_b] at h_trusted_read
+    rw [←BitVec.ofNatLT_eq_ofNat (w := 5) (n := Main[14].val) h_op_b_is_reg, h_read_op_b, Option.get!_some] at h_trusted_read
 
+    cases addr_cstr0
+    · sorry
+
+    rename_i h_has_shift
+    simp [h_has_shift] at chip_cstrs h_read_mem addr_cstr2
+
+    have h_mem_read_is_u64 : Word.isU64 #v[Main[29], Main[30], Main[31], Main[32]] := by simp_all only [chip_cstrs]
+
+    have h_over_addr : Main[26] ≠ 0 ∨ Main[27] ≠ 0 :=
+      by
+        by_contra!
+        clear * - addr_cstr1 this
+        obtain ⟨h_limb1_0, h_limb2_0⟩ := this
+        simp [h_limb1_0, h_limb2_0] at addr_cstr1
+    simp [not_and_or.mpr h_over_addr] at h_read_mem
+    obtain ⟨h_read_limb0, h_read_limb1, h_read_limb2, h_read_limb3⟩ := h_read_mem
+    
     simp [spec_lw, execute_LOAD]
 
     simp [Sail.readReg, PreSail.readReg, h_read_pc]
@@ -118,7 +139,7 @@ theorem correct
     simp [ext_data_get_addr]
     simp [op_b, sp1_op_b]
 
-    simp [Sail.writeReg, PreSail.writeReg, Sail.rX_bits_eq_get_reg?_no_run, h_read_op_b, Option.elim, Option.toSailM] 
+    simp [Sail.writeReg, PreSail.writeReg, Sail.rX_bits_eq_get_reg?_no_run, h_read_op_b, Option.elim, Option.toSailM]
 
     simp [check_misaligned, LeanRV64IM.Functions.plat_enable_misaligned_access, LeanRV64IM.Functions.not]
 
@@ -126,44 +147,192 @@ theorem correct
       simp [constraints, AddressOperation.constraints, AddrAddOperation.constraints, CPUState.constraints, ITypeReader.constraints, SP1Constraint.toProp, List.Forall, h_is_lw, h_not_lwu, Opcode.ofNat, ByteOpcode.ofNat, Nat.beq, Nat.ble] at cstrs
       simp_all only
 
-    -- TODO(gzgz): will come from `state_cstrs`
-    have h_trusted_aligned : ((s.get_reg? (BitVec.ofNat 5 Main[14].val)).get! + Word.toBitVec64 #v[Main[21], Main[22], Main[23], Main[24]]) % 4 = 0 := by sorry
-    rw [←BitVec.ofNatLT_eq_ofNat h_op_b_is_reg, h_read_op_b, h_op_c_is_signExtend, Option.get!_some] at h_trusted_aligned
-
     have h_is_aligned : is_aligned_vaddr (virtaddr.Virtaddr (Word.toBitVec64 #v[Main[15], Main[16], Main[17], Main[18]] + sign_extend op_c)) 4 = true := by
       unfold is_aligned_vaddr
       simp only [op_b, op_c, sp1_op_b, sp1_imm, sign_extend, Sail.BitVec.signExtend]
-      clear * - h_trusted_aligned
-      simp [BitVec.add_def, BitVec.umod_def, BitVec.ofNat, BitVec.ofNatLT] at h_trusted_aligned
-      -- simp [BitVec.add_def, Int.tmod_def]
+      rw [h_op_c_is_signExtend] at h_trusted_read
+      clear * - h_trusted_read
+      have := congrArg BitVec.toNat h_trusted_read
+      simp [-Word.toBitVec64_add_mod4, BitVec.toNat_umod, BitVec.ofNat_toNat] at this
       simp only [beq_iff_eq]
-      sorry
+      rw [←Int.ofNat_tmod]
+      -- praise Confucius this works
+      bv_omega
 
     simp [h_is_aligned, split_misaligned, bits_of_virtaddr]
-    
+
     simp [untilFuelM, untilFuelM.go, Sail.assert, PreSail.assert]
 
     simp [translateAddr]
     simp [Sail.readReg, PreSail.readReg, Std.ExtDHashMap.get?_insert, h_mstatus, h_priv]
     simp [effectivePrivilege, _get_Mstatus_MPRV, Sail.BitVec.extractLsb, translationMode]
 
-    clear * - h_mstatus h_priv mem0 mem1 mem2 mem3
+    -- clear * - h_mstatus h_priv mem0 mem1 mem2 mem3
 
-    have h_read_mem0 : s.mem[(Word.toBitVec64 #v[Main[15], Main[16], Main[17], Main[18]] + sign_extend op_c).toNat]? = some mem0 := by sorry
-    have h_read_mem1 : s.mem[(Word.toBitVec64 #v[Main[15], Main[16], Main[17], Main[18]] + sign_extend op_c).toNat + 1]? = some mem1 := by sorry
-    have h_read_mem2 : s.mem[(Word.toBitVec64 #v[Main[15], Main[16], Main[17], Main[18]] + sign_extend op_c).toNat + 2]? = some mem2 := by sorry
-    have h_read_mem3 : s.mem[(Word.toBitVec64 #v[Main[15], Main[16], Main[17], Main[18]] + sign_extend op_c).toNat + 3]? = some mem3 := by sorry
+    simp [ITypeReader.constraints, SP1Constraint.toProp, List.Forall, Opcode.ofNat, ByteOpcode.ofNat, Nat.ble, Nat.beq] at reader_cstrs
+    obtain ⟨h_add_addr_limb0, h_add_addr_limb1, h_add_addr_limb2, h_addr_add_spec⟩ :=
+      AddrAddOperation.correct
+      _ _ _ _ (by simp)
+      addr_add_cstrs
+      (by simp_all only [reader_cstrs])
+      (Word.isU64_of_cases _
+        (by simp; show Main[21] < 65536; simp_all only [reader_cstrs]) 
+        (by simp; show Main[22] < 65536; simp_all only [reader_cstrs]) 
+        (by simp; show Main[23] < 65536; simp_all only [reader_cstrs]) 
+        (by simp; show Main[24] < 65536; simp_all only [reader_cstrs]))
+      (by sorry) -- TODO(gzgz): not exceeding memory bounds, this should come from trusted_instr
+    simp at h_add_addr_limb0 h_add_addr_limb1 h_add_addr_limb2 h_addr_add_spec
+
+    -- TODO(gzgz): this will come from the cursed mod thingy
+    have h_addr_limb0_ge4 : Main[25] >= 4 :=
+      by
+        by_contra!
+        convert_to Main[25].val < 4 at this
+        simp [Fin.lt_def, Fin.mul_def, Fin.sub_def] at addr_cstr2
+        interval_cases Main[25].val
+        <;> simp at addr_cstr2
+
+    obtain ⟨h_limb2_mem0, h_limb2_mem1⟩ := h_read_limb2
+    have h_read_mem0 : s.mem[(Word.toBitVec64 #v[Main[15], Main[16], Main[17], Main[18]] + sign_extend op_c).toNat]? = some (BitVec.truncate 8 (BitVec.ofNat 16 ↑Main[31])) := by
+      simp only [op_c, sp1_imm, sign_extend, Sail.BitVec.signExtend]
+      rw [←h_op_c_is_signExtend]
+      rw [←h_addr_add_spec]
+      clear * - h_limb2_mem0 h_add_addr_limb0 h_add_addr_limb1 h_add_addr_limb2 h_addr_limb0_ge4
+      simp [-BitVec.toNat_ofNat, Word.toBitVec64, Word.toNat]
+      rw [←BitVec.ofNatLT_eq_ofNat (by omega)]
+      simp [BitVec.ofNatLT_toNat]
+      simp [Word.toNat] at h_limb2_mem0
+      simp [Fin.sub_val_of_le h_addr_limb0_ge4] at h_limb2_mem0
+      rw [←h_limb2_mem0]
+      apply congrArg
+      apply Eq.symm
+      calc 
+        _ = 4 + (↑Main[25] - 4 + _ + _) := by rw [add_comm (b := 4)]
+        _ = 4 + (↑Main[25] - 4) + _ + _ := by rw [←add_assoc, ←add_assoc]
+        _ = ↑Main[25] - 4 + 4 + _ + _ := by rw [add_comm (a := 4)]
+        _ = ↑Main[25] + 4 - 4 + _ + _ := by rw [←Nat.sub_add_comm (k := 4) h_addr_limb0_ge4]
+        _ = ↑Main[25] + (4 - 4) + _ + _ := by rw [Nat.add_sub_assoc (by simp)]
+        _ = ↑Main[25] + ↑Main[26] * 65536 + ↑Main[27] * 4294967296 := by simp
+
+    have h_read_mem1 : s.mem[(Word.toBitVec64 #v[Main[15], Main[16], Main[17], Main[18]] + sign_extend op_c).toNat + 1]? = some (BitVec.truncate 8 ((BitVec.ofNat 16 ↑Main[31]) >>> 8)) := by
+      simp only [op_c, sp1_imm, sign_extend, Sail.BitVec.signExtend]
+      rw [←h_op_c_is_signExtend]
+      rw [←h_addr_add_spec]
+      clear * - h_limb2_mem1 h_add_addr_limb0 h_add_addr_limb1 h_add_addr_limb2 h_addr_limb0_ge4
+      simp [-BitVec.toNat_ofNat, Word.toBitVec64, Word.toNat]
+      rw [←BitVec.ofNatLT_eq_ofNat (by omega)]
+      simp [BitVec.ofNatLT_toNat]
+      simp [Word.toNat] at h_limb2_mem1
+      simp [Fin.sub_val_of_le h_addr_limb0_ge4] at h_limb2_mem1
+      rw [←h_limb2_mem1]
+      apply congrArg
+      apply Eq.symm
+      sorry
+
+    have h_read_mem2 : s.mem[(Word.toBitVec64 #v[Main[15], Main[16], Main[17], Main[18]] + sign_extend op_c).toNat + 2]? = some (BitVec.truncate 8 ((BitVec.ofNat 16 ↑Main[32]))) := by sorry
+
+    have h_read_mem3 : s.mem[(Word.toBitVec64 #v[Main[15], Main[16], Main[17], Main[18]] + sign_extend op_c).toNat + 3]? = some (BitVec.truncate 8 (((BitVec.ofNat 16 ↑Main[32])) >>> 8)) := by sorry
+
+    have h_limb2_is_u16 : Main[31].val < 2^16 := h_mem_read_is_u64 2
+    have h_limb3_is_u16 : Main[32].val < 2^16 := h_mem_read_is_u64 3
+    simp only [←BitVec.ofNatLT_eq_ofNat h_limb2_is_u16, ←BitVec.ofNatLT_eq_ofNat h_limb3_is_u16] at h_read_mem0 h_read_mem1 h_read_mem2 h_read_mem3
 
     have h_always_within_ram : within_phys_mem (physaddr.Physaddr (Word.toBitVec64 #v[Main[15], Main[16], Main[17], Main[18]] + sign_extend op_c)) 4 = pure true := by
       sorry
 
     -- TODO(gzgz): comes from chip_cstrs
-    have h_op_a_not_x0 : op_a ≠ 0#5 := by sorry
+    have h_op_a_not_x0 : op_a ≠ 0#5 := by
+      simp [op_a, sp1_op_a, BitVec.ofNatLT, BitVec.ofNat]
+      have h_imm_c_is_0 : Main[13] = 0 := by simp_all only [chip_cstrs]
+      have h_imm_c_iff_op_a_x0 : Main[13] = 1 ↔ Main[6] = 0 := by simp_all only [reader_cstrs]
+      rw [Fin.mk_eq_mk]
+      simp
+      clear * - h_imm_c_is_0 h_imm_c_iff_op_a_x0
+      aesop
 
     simp [-BitVec.toNat_add, mem_read, Sail.readReg, PreSail.readReg, Std.ExtDHashMap.get?_insert, h_mstatus, h_priv, effectivePrivilege, _get_Mstatus_MPRV, Sail.BitVec.extractLsb, translationMode, mem_read_priv, mem_read_priv_meta, checked_mem_read, phys_access_check, bits_of_virtaddr, LeanRV64IM.Functions.sys_pmp_count, within_mmio_readable, get_config_rvfi, Sail.BitVec.addInt, zero_extend, Sail.BitVec.zeroExtend, h_always_within_ram, ext_check_phys_mem_read, phys_mem_read, read_kind_of_flags, read_ram, Sail.sail_mem_read, PreSail.sail_mem_read, PreSail.readBytes, PreSail.readByte, h_read_mem0, h_read_mem1, h_read_mem2, h_read_mem3, MemoryOpResult_drop_meta, h_op_a_not_x0]
 
     simp [misaligned_order, sys_misaligned_order_decreasing, extend_value, sign_extend, Sail.BitVec.signExtend]
+
+    simp [op_a] at h_op_a_not_x0
+    simp [sp1_lw, Sail.writeReg, PreSail.writeReg, Sail.write_reg, h_op_a_not_x0]
+
+    simp [Word.toBitVec64, Word.toNat]
+
+    have h_correct_limb0 : Main[39] = Main[31] := by simp_all only [chip_cstrs]
+    have h_correct_limb1 : Main[40] = Main[32] := by simp_all only [chip_cstrs]
+    rw [h_correct_limb0, h_correct_limb1]
+
+    have h_pc0 : Main[3].val < 65536 := by show Main[3] < 65536; simp_all only [reader_cstrs]
+    have h_pc1 : Main[4].val < 65536 := by show Main[4] < 65536; simp_all only [reader_cstrs]
+    have h_pc2 : Main[5].val < 65536 := by show Main[5] < 65536; simp_all only [reader_cstrs]
+
+    have h_pc_is_u64 : Main[3].val + Main[4].val * 65536 + Main[5].val * 4294967296 < 2^64 := by
+      simp
+      clear * - h_pc0 h_pc1 h_pc2
+      omega
+    rw [←BitVec.ofNatLT_eq_ofNat h_pc_is_u64]
+    simp [BitVec.add_def]
+
+    have : (↑(Main[3] + 4) + ↑Main[4] * 65536 + ↑Main[5] * 4294967296 : ℕ) = ↑Main[3] + ↑Main[4] * 65536 + ↑Main[5] * 4294967296 + 4 := by
+      simp [Fin.add_def]
+      rw [Nat.mod_eq_of_lt (by clear * - h_pc0; linarith)]
+      ring_nf
+    rw [this]
+    clear this
+    apply congrArg
+
+    simp [bitVecToRegidxVal]
+    simp [Sail.BitVec.updateSubrange, Sail.BitVec.updateSubrange', default]
     sorry
+
+lemma isprime : Nat.Prime 2013265921 := by native_decide
+
+instance : Lean.Grind.NoNatZeroDivisors (ZMod 2013265921) where
+  no_nat_zero_divisors := by
+    sorry
+
+lemma helper2
+  {x : Fin BB}
+  (hx : x < 65536)
+  (hmul : (x * 1761607681).val < 8192)
+  : x % 8 = 0
+  := by
+    convert_to x.val < 65536 at hx
+    simp [Fin.mod_def]
+    simp [Fin.mul_def, Fin.lt_def] at hmul
+
+    -- Use the Division Algorithm: x.val = 8 * q + r where 0 ≤ r < 8
+    set q := x.val / 8
+    set r := x.val % 8
+    have hx_eq : x.val = 8 * q + r := by
+      conv_lhs => rw [← Nat.div_add_mod x.val 8]
+    have hr_lt : r < 8 := Nat.mod_lt x.val (by norm_num : 0 < 8)
+
+    -- Key fact: 8 * 1761607681 ≡ 1 (mod BB)
+    have h_inv : (8 * 1761607681) % BB = 1 := by norm_num
+
+    have :=
+      calc ↑x * 1761607681 % BB = (8 * q + r) * 1761607681 % BB := by rw [hx_eq]
+                              _ = (8 * q * 1761607681 + r * 1761607681) % BB := by ring_nf
+                              _ = (8 * q * 1761607681 % BB + r * 1761607681) % BB := by simp
+                              _ = ((8 * 1761607681) * q % BB + r * 1761607681) % BB := by ring_nf
+                              _ = ((8 * 1761607681) % BB * q % BB + r * 1761607681) % BB := by rw [Nat.mod_mul_mod]
+                              _ = (1 * q % BB + r * 1761607681) % BB := by simp [BB]
+                              _ = (q % BB + r * 1761607681) % BB := by simp
+                              _ = (q + r * 1761607681) % BB := by simp
+    simp [BB] at this
+    rw [this] at hmul
+    clear this h_inv
+
+    -- Case on the 8 possible values of r
+    interval_cases r
+    -- Case r = 0
+    · rfl
+    -- Case 1 ≤ r < 8
+    all_goals 
+      simp at hmul
+      omega
 
 end LoadWord
 
